proof of OK case in asn_strtoimax_lim_correct until memory assumptions

src/C_strtoimax/Spec.v
@@ -7,160 +7,217 @@ Import ListNotations.
 Local Open Scope Int64Scope.
 
 Section Spec.
-  
-  (* Functional specification of INTEGER.c/asn_strtoimax_lim *)
-  
-  (* Informal spec:
-   
-    Parse the number in the given string until the given end position,
-    returning the position after the last parsed character back using the
-    same (end) pointer. WARNING: This behavior is different from the standard strtol/strtoimax(3).
-  *)
-  
-  (* Output type, see INTEGER.h  *)
-  
-  Inductive asn_strtox_result_e :=
-    | ASN_STRTOX_ERROR_RANGE (* Input outside of supported numeric range *)
-    | ASN_STRTOX_ERROR_INVAL (* Invalid data encountered (e.g., "+-") *)
-    | ASN_STRTOX_EXPECT_MORE (* More data expected (e.g. "+") *)
-    | ASN_STRTOX_EXTRA_DATA  (* Conversion succeded, but the string has extra stuff *)
-    | ASN_STRTOX_OK.         (* Conversion succeded, number ends at (end) *) 
-  
-  (* C light outputs directly int *)
-  
-  Definition asn_strtox_result_e_to_int (s : asn_strtox_result_e) : int :=
-    match s with
-      | ASN_STRTOX_ERROR_RANGE => Int.repr (-3)  
-      | ASN_STRTOX_ERROR_INVAL => Int.repr (-2)
-      | ASN_STRTOX_EXPECT_MORE => Int.repr (-1)
-      | ASN_STRTOX_EXTRA_DATA => Int.repr 1 
-      | ASN_STRTOX_OK => Int.repr 0
-    end.
-  
-  (* Useful notations and definitions *)
-  Definition minus_char := (Int.repr 45).
-  Definition plus_char := (Int.repr 43).
-  Definition zero_char := (Int.repr 48).
-  
-  (* Representing negative and positive int using signedness *)
-  Definition int_to_int64 (i : int) := Int64.repr (Int.signed i).
-  
-  Definition Sign s :=
-    match s with
-    | Signed => (Int.repr (-1))
-    | Unsigned => Int.repr 1
-    end.
 
-  Definition sign i :=
-    if (i == minus_char)%int then Signed else Unsigned.
-  
-  Definition mult_sign s value :=
-    match s with
-    | Signed =>  ((Int64.repr (-1))*value)%int64 
-    | Unsigned => value
-    end.
-  
- (* Converting a single char into into a number given previous value *)   
-  Definition digit_to_num s i v :=
-    match s with
-    | Signed => (Int64.neg v * (Int64.repr 10) -
+(* Functional specification of INTEGER.c/asn_strtoimax_lim *)
+
+(* Informal spec:
+
+  Parse the number in the given string until the given end position,
+  returning the position after the last parsed character back using the
+  same (end) pointer. WARNING: This behavior is different from the standard strtol/strtoimax(3).
+*)
+
+(* Output type, see INTEGER.h  *)
+
+Inductive asn_strtox_result_e :=
+  | ASN_STRTOX_ERROR_RANGE (* Input outside of supported numeric range *)
+  | ASN_STRTOX_ERROR_INVAL (* Invalid data encountered (e.g., "+-") *)
+  | ASN_STRTOX_EXPECT_MORE (* More data expected (e.g. "+") *)
+  | ASN_STRTOX_EXTRA_DATA  (* Conversion succeded, but the string has extra stuff *)
+  | ASN_STRTOX_OK.         (* Conversion succeded, number ends at (end) *)
+
+(* C light outputs directly int *)
+
+Definition asn_strtox_result_e_to_int (s : asn_strtox_result_e) : int :=
+  match s with
+    | ASN_STRTOX_ERROR_RANGE => Int.repr (-3)
+    | ASN_STRTOX_ERROR_INVAL => Int.repr (-2)
+    | ASN_STRTOX_EXPECT_MORE => Int.repr (-1)
+    | ASN_STRTOX_EXTRA_DATA => Int.repr 1
+    | ASN_STRTOX_OK => Int.repr 0
+  end.
+
+(* Useful notations and definitions *)
+Definition minus_char := (Int.repr 45).
+Definition plus_char := (Int.repr 43).
+Definition zero_char := (Int.repr 48).
+
+(* Representing negative and positive int using signedness *)
+Definition int_to_int64 (i : int) := Int64.repr (Int.signed i).
+
+Definition Sign s :=
+  match s with
+  | Signed => (Int.repr (-1))
+  | Unsigned => Int.repr 1
+  end.
+
+Definition sign i :=
+  if (i == minus_char)%int then Signed else Unsigned.
+
+Definition mult_sign s value :=
+  match s with
+  | Signed =>  ((Int64.repr (-1))*value)%int64
+  | Unsigned => value
+  end.
+
+(* Converting a single char into into a number given previous value *)
+Definition digit_to_num s i v :=
+  match s with
+  | Signed => (Int64.neg v * (Int64.repr 10) -
+               int_to_int64 (i - zero_char)%int)
+  | Unsigned => (v * (Int64.repr 10) +
                  int_to_int64 (i - zero_char)%int)
-    | Unsigned => (v * (Int64.repr 10) +
-                   int_to_int64 (i - zero_char)%int)
-    end.
-      
-  (* Memory, global and local env are fixed *)
-  Variable m : mem.
-  Variable ge : genv.
-  Variable e : env.
+  end.
 
-  (* Constants of the function *)
-  Definition ASN1_INTMAX_MAX := (Int64.not 0) >> 1.
-  Definition upper_boundary := ASN1_INTMAX_MAX // (Int64.repr 10).
-  Definition last_digit_max := ASN1_INTMAX_MAX % (Int64.repr 10).
-  Definition last_digit_max_minus := (ASN1_INTMAX_MAX % (Int64.repr 10)) + 1.
+(* Memory, global and local env are fixed *)
+Variable m : mem.
+Variable ge : genv.
+Variable e : env.
 
-  Definition max_sign s :=
-    match s with
-    | Signed => last_digit_max_minus 
-    | Unsigned => last_digit_max
-    end.
-  
-  (* digits [0-9]*)
-  Definition digits := map Int.repr [48;49;50;51;52;53;54;55;56;57].
-  Definition is_digit (i : int) := existsb (fun j => Int.eq i j) digits.
-  
-  (* Executable spec *)
+(* Constants of the function *)
+Definition ASN1_INTMAX_MAX := (Int64.not 0) >> 1.
+Definition upper_boundary := ASN1_INTMAX_MAX // (Int64.repr 10).
+Definition last_digit_max := ASN1_INTMAX_MAX % (Int64.repr 10).
+Definition last_digit_max_minus := (ASN1_INTMAX_MAX % (Int64.repr 10)) + 1.
 
-  (* Return type *)
-  Record asn_strtoimax_lim_result :=
-    { return_type : asn_strtox_result_e ;
-      value : option int64 ;
-      memory : option mem ; 
-      }.
-  
-  Fixpoint asn_strtoimax_lim_loop (str fin intp : addr) (value : int64) (s: signedness) (last_digit : int64) (dist : nat) (m'' : mem) {struct dist} : option asn_strtoimax_lim_result :=
-    match dist with
-    | O => match (Mem.storev Mptr m'' (vptr fin) (vptr str)) with
-          | Some m' => 
-            Some {| return_type := ASN_STRTOX_OK;
-                    value := Some (mult_sign s value);
-                    memory := Mem.storev Mint64 m' (vptr intp) (Vlong (mult_sign s value)) |}
-          | None => None
-          end        
-    | S n => match load_addr Mint8signed m'' str with
-            | Some (Vint i) =>
-              if is_digit i
-              then let d := int_to_int64 (i - zero_char)%int in
-                   if value < upper_boundary
-                   then asn_strtoimax_lim_loop (str++) fin intp
-                        (value * (Int64.repr 10) + d) s last_digit n m
-                   else if (value == upper_boundary) && (d <= last_digit)
-                        then  asn_strtoimax_lim_loop (str++) fin intp
-                                   (digit_to_num s i value) s last_digit n m
-                        else match (Mem.storev Mptr m'' (vptr fin) (vptr str)) with
-                             | Some m' => 
-                               Some {| return_type := ASN_STRTOX_ERROR_RANGE;
-                                       value := None;
-                                       memory := Some m' |}
-                             | None => None
-                             end                          
-              else match (Mem.storev Mptr m'' (vptr fin) (vptr str)) with
-                   | Some m' => Some {| return_type := ASN_STRTOX_EXTRA_DATA;
-                                       value := Some (mult_sign s value);
-                                       memory := Mem.storev Mint64 m' (vptr intp) (Vlong (mult_sign s value)) |}
-                   | None => None
+Definition max_sign s :=
+  match s with
+  | Signed => last_digit_max_minus
+  | Unsigned => last_digit_max
+  end.
+
+(* digits [0-9]*)
+Definition is_digit (i : int) := andb ((Int.repr 48) <= i)%int ( i <= (Int.repr 57))%int.
+
+(* Executable spec *)
+
+(* Return type *)
+Record asn_strtoimax_lim_result :=
+  { return_type : asn_strtox_result_e ;
+    value : option int64 ;
+    memory : option mem ;
+    }.
+
+
+Fixpoint asn_strtoimax_lim_loop (str fin intp : addr) (value : int64)
+         (s: signedness) (last_digit : int64)
+         (dist : nat) (m'' : mem) {struct dist} : option asn_strtoimax_lim_result :=
+  match dist with
+  | O => Some {| return_type := ASN_STRTOX_OK;
+                  value := Some (mult_sign s value);
+                  memory := Some m'' |}
+  | S n => match load_addr Mint8signed m'' str with
+           | Some (Vint i) =>
+            if is_digit i
+            (* if *str >= 0x30 && *str <= 0x39 *)
+            then let d := int_to_int64 (i - zero_char)%int in
+                 (* int d = *str - '0' *)
+                 if value < upper_boundary
+                 then asn_strtoimax_lim_loop (str++) fin intp
+                      (value * (Int64.repr 10) + d) s last_digit n m
+                      (* value = value * 10 + d; next iteration *)
+                 else if (value == upper_boundary) && (d <= last_digit_max)
+                      (* firstly check if str < *end, and if so, return *)
+                      then let value' := digit_to_num s i value in
+                           let s' := match s with | Signed => Unsigned | _ => Unsigned end in
+                           let str' := (str++) in
+                           match (Mem.loadv Mptr m'' (vptr fin)) with
+                           | Some (Vptr b fin') =>
+                             if (addr_lt m'' str' (b, fin'))
+                             then match (Mem.storev Mptr m'' (vptr fin) (vptr str)) with
+                                  (* *end = str *)
+                                  | Some m' => match (load_addr Mint8signed m'' str) with
+                                              | Some (Vint i') =>
+                                                if is_digit i'
+                                                (* if *str >= 0x30 && *str <= 0x39 *)
+                                                then Some {|
+                                                         return_type := ASN_STRTOX_ERROR_RANGE;
+                                                         value := None;
+                                                         memory := Some m' |}
+                                                else Some {|
+                                                         return_type := ASN_STRTOX_EXTRA_DATA;
+                                                         value := Some (mult_sign s' value');
+                                                         memory := Mem.storev Mint64 m' (vptr intp)
+                                                                    (Vlong (mult_sign s' value')) |}
+                                              | _ => None
+                                              end
+                                  | None => None
+                                  end
+                             else
+                               Some {| return_type := ASN_STRTOX_OK;
+                                            value := Some (mult_sign s value);
+                                            memory := Some m'' |}
+                             (* if str > *end, then we break the loop *)
+                           | _ => None
+                           end
+                      else match (Mem.storev Mptr m'' (vptr fin) (vptr str)) with
+                           | Some m' =>
+                             Some {| return_type := ASN_STRTOX_ERROR_RANGE;
+                                     value := None;
+                                     memory := Some m' |}
+                           | None => None
+                           end
+            else match (Mem.storev Mptr m'' (vptr fin) (vptr str)) with
+                 | Some m' => Some {| return_type := ASN_STRTOX_EXTRA_DATA;
+                                     value := Some (mult_sign s value);
+                                     memory := Mem.storev Mint64 m' (vptr intp)
+                                                          (Vlong (mult_sign s value)) |}
+                 | None => None
+                 end
+          | _ => None
+          end
+  end.
+
+Definition store_result str fin intp res :=
+  match res with
+  | Some {| return_type := ASN_STRTOX_OK;
+            value := Some val;
+            memory := Some m'; |} =>
+    match (Mem.storev Mptr m' (vptr fin) (vptr str)) with
+    | Some m'' =>
+      Some {| return_type := ASN_STRTOX_OK;
+              value := Some val;
+              memory := Mem.storev Mint64 m'' (vptr intp)
+                                   (Vlong val) |}
+    | None => None
+    end
+  | _ => res
+  end.
+    
+Definition asn_strtoimax_lim (str fin intp : addr) : option asn_strtoimax_lim_result :=
+  match load_addr Mptr m fin with (* derefencing **fin *)
+  | Some (Vptr b ofs) =>
+    match addr_ge m str (b, ofs) with (* compare str and *fin *)
+    | Some true => Some {| return_type := ASN_STRTOX_ERROR_INVAL;
+                                           value := None;
+                                           memory := Some m; |}
+    | Some false => let dist := distance str (b,ofs) in
+                   match load_addr Mint8signed m str with
+                   | Some (Vint i) =>
+                     if (i == minus_char)%int || (i == plus_char)%int
+                     then match addr_ge m (str++) (b,ofs) with
+                          | Some true =>
+                            Some {| return_type := ASN_STRTOX_EXPECT_MORE;
+                                    value := None;
+                                    memory := (Mem.storev Mptr m
+                                                          (vptr fin)
+                                                          (vptr (str++))); |}
+
+                          | Some false => store_result (str++) fin intp
+                                           (asn_strtoimax_lim_loop
+                                           (str++) fin intp 0 (sign i)
+                                           (max_sign (sign i)) (dist - 1)%nat m)
+                          | None => None
+                          end
+                     else store_result str fin intp
+                            (asn_strtoimax_lim_loop str fin intp 0
+                                Unsigned last_digit_max dist m)
+                   | _ => None (* fail of memory load on str: wrong type or not enough permission *)
                    end
-            | _ => None                
-            end
-    end.
-
-  Definition asn_strtoimax_lim (str fin intp : addr) : option asn_strtoimax_lim_result :=
-    match load_addr Mptr m fin with (* derefencing **fin *)
-    | Some (Vptr b ofs) =>
-      match addr_ge m str (b, ofs) with (* compare str and *fin *)
-      | Some true => Some {| return_type := ASN_STRTOX_ERROR_INVAL;
-                                             value := None;
-                                             memory := Some m; |}
-      | Some false => let dist := distance str (b,ofs) in
-                     match load_addr Mint8signed m str with
-                     | Some (Vint i) =>
-                       if (i == minus_char)%int || (i == plus_char)%int
-                       then match addr_ge m (str++) (b,ofs) with
-                            | Some true =>  Some {| return_type := ASN_STRTOX_EXPECT_MORE;
-                                             value := None;
-                                             memory := (Mem.storev Mptr m (vptr fin) (vptr (str++))); |}
-  
-                            | Some false => asn_strtoimax_lim_loop (str++) fin intp 0 (sign i) (max_sign (sign i)) (dist - 1)%nat m
-                            | None => None
-                            end
-                        else asn_strtoimax_lim_loop str fin intp 0 Unsigned last_digit_max dist m
-                     | _ => None (* fail of memory load on str: wrong type or not enough permission *)
-                     end
-      | None => None (* error in pointer comparison *)
-      end 
-    | _ => None (* fail of pointer to fin *) 
-    end.
+    | None => None (* error in pointer comparison *)
+    end
+  | _ => None (* fail of pointer to fin *)
+  end.
 
 (* Abstract specification *)
 (* Z or int? *)
@@ -186,7 +243,7 @@ Definition string_to_int (s : list int) (sign : signedness) :
                   then string_to_int_loop tl sign
                                           (digit_to_num sign char v)
                   else (Some (digit_to_num sign char v),
-                        ASN_STRTOX_EXTRA_DATA)                      
+                        ASN_STRTOX_EXTRA_DATA)
     end
   in string_to_int_loop s sign 0.
 
@@ -200,7 +257,7 @@ Fixpoint string_at_address (s : list int) str dist : option (list int) :=
           | _ => None
           end
   end.
-(*    
+(*
 Proposition asn_strtoimax_lim_fun_correct :
   forall dist str_b str_ofs fin_b fin_ofs intp_b intp_ofs m' val sign s,
       dist = distance (str_b, str_ofs) (fin_b, fin_ofs) ->
@@ -208,7 +265,7 @@ Proposition asn_strtoimax_lim_fun_correct :
       string_to_int s sign = val ->
       m' = Mem.store Mint64 m intp_b (Ptrofs.unsigned intp_ofs)
                      (Vlong (mult_sign sign val)) ->
-      
+
     asn_strtoimax_lim_loop (str_b, str_ofs) (fin_b, fin_ofs) (intp_b, intp_ofs)
                            0 sign (max_sign sign) dist m =
     Some {| return_type := ASN_STRTOX_OK ;
@@ -224,7 +281,7 @@ Proof.
   break_match.
   rewrite <- H1.
   econstructor.
-    
+
   unfold asn_strtoimax_lim.
   repeat break_match; try congruence.
   intros.
